Veritas.Verifier.Merkle.fst
@@ -1,0 +1,8 @@
+module Veritas.Verifier.Merkle
+
+open Veritas.BinTreePtr
+open Veritas.EAC
+open Veritas.Verifier
+open Veritas.Verifier.CorrectDefs
+
+let eac_ptrfn (#n:nat) (itsl: its_log n): ptrfn = admit()
